Work in progress on stackability, modifications in the module structure

Eval.v
@@ -5,132 +5,182 @@ Require Import List.
 Import ListNotations.
 Open Scope nat_scope.
 
-Check fold_left.
-
-Definition assign (v0: Value) (x: Var) (v: Value) (σ: Store) : Store :=
-  match (getObj σ v0) with
+Module Evaluator.
+  Parameter ct: ClassTable.
+  
+  Definition assign (v0: Value) (x: Var) (v: Value) (σ: Store) : Store :=
+    match (getObj σ v0) with
     | Some (C, fields) => [ v0 ↦ (C, [x ↦ v]fields)] σ
     | None => σ (* ? *)
-  end.
+    end.
 
-Definition assign_list (v0: Value) (x: list Var) (v: list Value) (σ: Store) : Store :=
-  match (getObj σ v0) with
+  Definition assign_list (v0: Value) (x: list Var) (v: list Value) (σ: Store) : Store :=
+    match (getObj σ v0) with
     | Some (C, fields) => [v0 ↦ (C, [x ⟼ v]fields)] σ
     | None => σ
-  end.
+    end.
 
-Reserved Notation "'⟦' e '⟧' '(' ct ',' σ ',' ρ ',' v ')(' k ')'"   (at level 200).
-Reserved Notation "'⟦_' e '_⟧' '(' ct ',' σ ',' ρ ',' v ')(' k ')'" (at level 200).
+  Reserved Notation "'⟦' e '⟧' '(' σ ',' ρ ',' v ')(' k ')'"   (at level 80).
+  Reserved Notation "'⟦_' e '_⟧' '(' σ ',' ρ ',' v ')(' k ')'" (at level 80).
 
-Fixpoint eval (e: Expr) (ct: ClassTable) (σ: Store) (ρ: Env) (v: Value) (k: nat) : Result :=
-  match k with
-  | 0 => Timeout
-  | S n => match e with
-          (* Var: simple lookup of the store *)
-          | var x => (
-              match (getVal ρ x) with
-              | Some v => (Success v σ)
-              | _ => Error
-              end )
+  Fixpoint eval (e: Expr) (σ: Store) (ρ: Env) (v: Value) (k: nat) : Result :=
+    match k with
+    | 0 => Timeout
+    | S n => match e with
+            (* Var: simple lookup of the store *)
+            | var x => (
+                match (getVal ρ x) with
+                | Some v => (Success v σ)
+                | _ => Error
+                end )
 
-          (* This: returns current value *)
-          | this => (Success v σ) 
+            (* This: returns current value *)
+            | this => (Success v σ) 
 
-          (* Field access: compute object value and access field *)
-          | fld e0 x => (
-              match (⟦e0⟧(ct, σ, ρ, v)(n)) with
-              | Success v0 σ1 =>
-                match (getObj σ1 v0) with
-                | Some (c, f) =>
-                  match (getVal f x) with
-                  | Some v1 => Success v1 σ1
-                  | _ => Error end
-                | _ => Error end
-              | _ => Error end )
-
-          (* Method call : compute object value, compute arguments and do the call*)
-          | mtd e0 m e_l => (
-              match (⟦e0⟧(ct, σ, ρ, v)(n)) with
-              | Success v0 σ1 => (
+            (* Field access: compute object value and access field *)
+            | fld e0 x => (
+                match (⟦e0⟧(σ, ρ, v)(n)) with
+                | Success v0 σ1 =>
                   match (getObj σ1 v0) with
-                   | Some (C, _) => (
-                       match (ct C)  with
+                  | Some (c, f) =>
+                    match (getVal f x) with
+                    | Some v1 => Success v1 σ1
+                    | _ => Error end
+                  | _ => Error end
+                | _ => Error end )
+
+            (* Method call : compute object value, compute arguments and do the call*)
+            | mtd e0 m el => (
+                match (⟦e0⟧(σ, ρ, v)(n)) with
+                | Success v0 σ1 => (
+                    match (getObj σ1 v0) with
+                    | Some (C, _) => (
+                        match (ct C)  with
                         | Some (class _  _ methods) => (
                             match methods m with
-                             | Some (method μ x _ e1) => (
-                                match (⟦_ e_l _⟧(ct, σ1, ρ, v)(n)) with
-                                 | Success_list args_val σ2 => let ρ1 := [(removeTypes x) ⟼ args_val]∅ in
-                                                           ⟦e1⟧(ct, σ2, ρ1, v)(n)
-                                 | _ => Error end)
+                            | Some (method μ x _ e1) => (
+                                match (⟦_ el _⟧(σ1, ρ, v)(n)) with
+                                | Success_list args_val σ2 => let ρ1 := [(removeTypes x) ⟼ args_val]∅ in
+                                                             ⟦e1⟧(σ2, ρ1, v)(n)
+                                | _ => Error end)
                             | _ => Error end)
-                       | _ => Error end)
-                   | _ => Error end)
-              | _ => Error end)
-                             
-          (* New class *)
-          | new C args => (
-              match (⟦_ args _⟧(ct, σ, ρ, v)(n)) with
+                        | _ => Error end)
+                    | _ => Error end)
+                | _ => Error end)
+                               
+            (* New class *)
+            | new C args => (
+                match (⟦_ args _⟧(σ, ρ, v)(n)) with
                 | Success_list args_val σ1 => (
                     let I := (length σ1) + 1 in
                     let σ2 := [I ↦ (C, ∅)] σ1 in (
-                    match (init I args_val C ct σ2 n) with
+                      match (init I args_val C σ2 n) with
                       | Some σ3 => (Success I σ3)
                       | None => Error end ))
                 | _ => Error end) (* Unknown class *) 
 
-          (* Field assignement *)
-          | asgn e1 x e2 e' => (
-              match (⟦e1⟧(ct, σ, ρ, v)(n)) with
-                | Success v1 σ1 => match (⟦e2⟧(ct, σ1, ρ, v)(n)) with
-                                    | Success v2 σ2 => (
-                                        let σ3 := (assign v1 x v2 σ2) in
-                                        ⟦e'⟧(ct, σ3, ρ, v)(n))
-                                    | _ => Error end
+            (* Field assignement *)
+            | asgn e1 x e2 e' => (
+                match (⟦e1⟧(σ, ρ, v)(n)) with
+                | Success v1 σ1 => match (⟦e2⟧(σ1, ρ, v)(n)) with
+                                  | Success v2 σ2 => (
+                                      let σ3 := (assign v1 x v2 σ2) in
+                                      ⟦e'⟧(σ3, ρ, v)(n))
+                                  | _ => Error end
                 | _ => Error end ) 
-          end
-  end
-where "'⟦' e '⟧' '(' ct ',' σ ',' ρ ',' v ')(' k ')'" := (eval e ct σ ρ v k)
-with eval_list (e_l: list Expr) (ct: ClassTable) (σ: Store) (ρ: Env) (v: Value) (k: nat) :  Result :=
-   match k with
-     | 0 => Timeout
-     | S n => fold_left (eval_list_aux ct σ ρ v n) e_l (Success_list [] σ) end
-where "'⟦_' e '_⟧' '(' ct ',' σ ',' ρ ',' v ')(' k ')'" := (eval_list e ct σ ρ v k)
-with eval_list_aux (ct: ClassTable) (σ: Store) (ρ: Env) (v: Value) (k: nat) (acc: Result) (e: Expr) :=
-   match k with
-     | 0 => Timeout
-     | S n => match acc with
-       | Success_list vs σ1 => match (⟦e⟧(ct, σ1, ρ, v)(n)) with
-                              | Success v σ2 => Success_list (v::vs) σ2
-                              | z => z end
-       | z => z end end
-with init (I : Var) (v : list Var) (C: ClN) (ct: ClassTable) (σ: Store) (k :nat) : option Store :=
-   match k with
-     | 0 => None
-     | S n =>
-       match (ct C) with
-         | Some (class x F M) => (
-             let σ1 := (assign_list I (removeTypes x) v σ) in
-             let f  := (fun (σ: Store) (f: Field) => match f with
-                          |field x t e => (
-                             match (⟦e⟧(ct, σ, ∅, I)(n)) with
-                               | Success v1 σ1 => (assign I x v1 σ1)
-                               | _ => σ (* In case or error, we keep σ to help for some proofs *)
-                             end) end) in
-             Some (fold_left f F σ)) 
-         | None => None
-       end
-   end.
+            end 
+    end 
+  where "'⟦' e '⟧' '(' σ ',' ρ ',' v ')(' k ')'"  := (eval e σ ρ v k)
+  with eval_list (e_l: list Expr) (σ: Store) (ρ: Env) (v: Value) (k: nat) :  Result :=
+         match k with
+         | 0 => Timeout
+         | S n => fold_left (eval_list_aux σ ρ v n) e_l (Success_list [] σ) end
+  where  "'⟦_' e '_⟧' '(' σ ',' ρ ',' v ')(' k ')'" := (eval_list e σ ρ v k)
+  with eval_list_aux (σ: Store) (ρ: Env) (v: Value) (k: nat) (acc: Result) (e: Expr) :=
+         match k with
+         | 0 => Timeout
+         | S n => match acc with
+                 | Success_list vs σ1 => match (⟦e⟧(σ1, ρ, v)(n)) with
+                                        | Success v σ2 => Success_list (v::vs) σ2
+                                        | z => z end
+                 | z => z end end
+  with init (I : Var) (v : list Var) (C: ClN) (σ: Store) (k :nat) : option Store :=
+         match k with
+         | 0 => None
+         | S n =>
+           match (ct C) with
+           | Some (class x F M) => (
+               let σ1 := (assign_list I (removeTypes x) v σ) in
+               let f  := (fun (σ: Store) (f: Field) => match f with
+                                                    |field x t e => (
+                                                       match (⟦e⟧(σ, ∅, I)(n)) with
+                                                       | Success v1 σ1 => (assign I x v1 σ1)
+                                                       | _ => σ (* In case or error, we keep σ to help for some proofs *)
+                                                       end) end) in
+               Some (fold_left f F σ)) 
+           | None => None
+           end
+         end.
 
 
 
-Lemma eval_not_success_list: forall  (k: nat) (e: Expr) (ct: ClassTable) (σ σ': Store) (ρ: Env) (v: Value) (l: list Value),
-    not (⟦e⟧(ct, σ, ρ, v)(k) = Success_list l σ').
-  induction k => //.
-  intros.
-  destruct e => //.
-  - simpl. destruct (getVal ρ v0) => //.
-  - simpl. destruct (⟦ e ⟧ (ct, σ, ρ, v )( k)) => //. destruct (getObj s v1) => //. destruct o => //. destruct (getVal e0 v0) => //.
-  - simpl. destruct (⟦ e ⟧ (ct, σ, ρ, v )( k)) => //. destruct (getObj s v0) => //. destruct o => //. destruct (ct c) => //. destruct c0 => //. destruct (methods m) => //. destruct m0 => //. destruct (⟦_ l0 _⟧ (ct, s, ρ, v )( k)) => //.
-  - simpl. destruct (⟦_ l0 _⟧ (ct, σ, ρ, v )( k)) => //. destruct (init (length s + 1) l1 c ct [length s + 1 ↦ (c, [])] (s) k) => //.
-  - simpl. destruct (⟦ e1 ⟧ (ct, σ, ρ, v )( k)) => //. destruct (⟦ e2 ⟧ (ct, s, ρ, v )( k)) => //.
-Qed.  
+  Lemma eval_not_success_list: forall  (k: nat) (e: Expr) (σ σ': Store) (ρ: Env) (v: Value) (l: list Value),
+      not (⟦e⟧(σ, ρ, v)(k) = Success_list l σ').
+    induction k => //.
+    intros.
+    destruct e => //.
+    - simpl.
+      destruct (getVal ρ v0) => //.
+    - simpl.
+      destruct (⟦ e ⟧ (σ, ρ, v )( k)) => //.
+      destruct (getObj s v1) => //.
+      destruct o => //.
+      destruct (getVal e0 v0) => //.
+    - simpl.
+      destruct (⟦ e ⟧ (σ, ρ, v )( k)) => //.
+      destruct (getObj s v0) => //.
+      destruct o => //.
+      destruct (ct c) => //.
+      destruct c0 => //.
+      destruct (methods m) => //.
+      destruct m0 => //.
+      destruct (⟦_ l0 _⟧ ( s, ρ, v )( k)) => //.
+    - simpl.
+      destruct (⟦_ l0 _⟧ (σ, ρ, v )( k)) => //.
+      destruct (init (length s + 1) l1 c [length s + 1 ↦ (c, [])] (s) k) => //.
+    - simpl.
+      destruct (⟦ e1 ⟧ (σ, ρ, v )( k)) => //.
+      destruct (⟦ e2 ⟧ (s, ρ, v )( k)) => //.
+  Qed.
+
+
+  (*
+  Lemma eval_preserves_types: forall (k: nat) (e: Expr) (σ σ': Store) (ρ ω ω': Env) (v v': Value) (l: Loc) (C C': ClN),
+      (⟦e⟧(σ, ρ, v)(k) = Success v' σ') ->
+      (getObj σ l) = Some (C, ω) ->
+      (getObj σ' l) = Some (C', ω') -> C=C'.
+    induction k => //.
+    destruct e; simpl ; intros.
+    - destruct (getVal ρ v) => //.
+      injection H => H2 H3.
+      rewrite -H2 in H1.
+      rewrite H0 in H1.
+      injection H1  => //.
+    - injection H => H2 H3.
+      rewrite -H2 in H1.
+      rewrite H0 in H1.
+      injection H1  => //.
+    - destruct (⟦ e ⟧ (σ, ρ, v0 )( k)) eqn:E => //.
+      destruct (getObj s v1) eqn:S => //.
+      destruct o => //.
+      destruct (getVal e0 v) => //.
+      injection H => H2 H3.
+      rewrite -H2 in H1.
+      apply : (IHk e σ s ρ ω ω' v0 v1 l C C' E H0 H1).
+    -  Admitted.      
+*)      
+    
+      
+  
+
+  End Evaluator.
