Stackability.v
@@ -1,0 +1,61 @@
+From Celsius Require Export Trees.
+From Celsius Require Export Eval.
+From Celsius Require Export PartialMonotonicity.
+From Celsius Require Export Reachability.
+Require Import ssreflect ssrbool.
+
+
+
+Module Reachability.
+  Import Eval.Evaluator.
+  Import Reachability.Reachability.
+  Import PartialMonotonicity.PartialMonotonicity.
+  
+  Definition stackability (σ σ' : Store) :=
+    forall l, l < (dom σ') -> ((σ' ⊨ l : warm) \/ (l < (dom σ))).
+  Notation "σ ≪ σ'" := (stackability σ σ') (at level 80).
+  
+  Lemma stackability_reflexivity: forall σ, σ ≪ σ.
+  Proof.
+    unfold stackability. right => //.
+  Qed.
+
+  Lemma stackability_transitivity: forall σ1 σ2 σ3,
+      σ1 ≪ σ2 -> σ2 ≪ σ3 -> σ2 ⪯ σ3 -> σ1 ≪ σ3.
+  Proof.
+    unfold stackability.
+    intros.
+    case /(_ l H2):H0 => H0.
+    - left => //.
+    - case /(_ l H0):H => H.
+      + left. apply: (partialMonotonicity_warm_monotone σ2 σ3 l H1 H) => //.
+      + right => //.
+  Qed.      
+
+  Lemma stackability_assignment : forall (σ σ': Store) (l l': Loc) (C: ClN) (f: Value) (ω ω': Env),
+      (getObj σ l) = Some (C, ω) ->
+      ω' = [f ↦ l']ω ->
+      σ' = [l ↦ (C, ω')]σ ->
+      σ ≪ σ'.
+  Proof.
+    unfold stackability, dom.
+    intros.
+    right.
+    move: (update_one3 _ l (C,ω') σ).
+    rewrite -H1 => H3.
+    rewrite -H3 => //.
+  Qed.
+
+
+
+    
+
+
+    
+
+  
+    
+    
+      
+    
+
